% !TEX root = ../*.tex
Show that  for $R \sim Bin(\pi, m)$, $K_{Bin}(t)$ the cumulant generating function $\log(M_{Bin}(t))$ is $m\log(1-\pi +\pi e^t)$. 

We will start by deriving the MGF of the Binomial distribution, \\${M_{Bin}(t) = (1-\pi +\pi e^t)^m}$.
\begin{align*}
    M_{Bin}(t) &= \expec{e^{Rt}} = \sum_{x=0}^m e^{xt}\cdot P(R=x)\\ 
               &=\sum_{y=0}^m e^{xt} {m \choose x}\pi^x(1-\pi)^{m-x}\\
                 &=\sum_{y=0}^m  {m \choose x} (e^t \pi)^x(1-\pi)^{m-x}\\
\end{align*}
Recall from the Binomial Theorem that:
\begin{equation}
    \label{bin_thm}
    (z+y)^n = \sum_{k=0}^n{n \choose k}z^{k}y^{n-k} = \sum_{k=0}^n{n \choose k}z^{n-k}y^{k}
\end{equation}
By choosing $z := e^t \pi$, $y:= 1 - \pi$, $k:=x$, and $m:=n$, we have that:

\begin{align*}
    \sum_{y=0}^m  {m \choose x} (e^t \pi)^x(1-\pi)^{m-x} = (\pi e^t + 1-\pi)^m\\
\end{align*}
Thus, 
\begin{align*}
    K_{Bin}(t) = log(M_{bin}(t) =  m\log(\pi e^t + 1-\pi)\\
    \blacksquare
\end{align*}


