\prompt{Show that $\expec{\xi({\vec{\theta}})}= \frac{\vec{y}_0}{\lambda} + c$ and 
$\expec{\xi({\vec{\theta}})|\samp{\vec{y}}}= \frac{\vec{y}_0+n\vec{\bar{y}}}{\lambda+n}+c$ for some constanct $c$}

Using the hint and the result from part a, we have:
\begin{align*}
    \expec{\xi({\vec{\theta}})} = \expec{\partiald{\psi(\theta)}{\vec{\theta}}} 
    &= \expec{\partiald{\psi(\theta)}{\vec{\theta}}}\\
    &= \expec{\frac{1}{\lambda}\Big(\vec{y}_0- \Big(\vec{y}_0-\lambda\partiald{\psi(\vec{\theta})}{\vec{\theta}}\Big)\Big)}\\
    &= \expec{\frac{1}{\lambda}\Big(\vec{y}_0- 
    \frac{\partiald{}{\vec{\theta}}\exp(\vec{\theta}\tp\vec{y}_0 - \lambda\psi(\vec{\theta}))}{\exp(\vec{\theta}\tp\vec{y}_0 - \lambda\psi(\vec{\theta}))}\Big)}\\
    &= \frac{1}{\lambda}\Big(\vec{y}_0- 
    \expec{\frac{\partiald{}{\vec{\theta}}\exp(\vec{\theta}\tp\vec{y}_0 - \lambda\psi(\vec{\theta}))}{\exp(\vec{\theta}\tp\vec{y}_0 - \lambda\psi(\vec{\theta}))}}\Big)\\
    &= \frac{1}{\lambda}\Big(\vec{y}_0- 
    \int{\frac{\partiald{}{\vec{\theta}}\exp(\vec{\theta}\tp\vec{y}_0 - \lambda\psi(\vec{\theta}))}
{\exp(\vec{\theta}\tp\vec{y}_0 - \lambda\psi(\vec{\theta}))}h(\vec{y}_0,\lambda)\exp(\vec{\theta}\tp\vec{y}_0 - \lambda\psi(\vec{\theta}))d\vec{\theta}}\Big)\\
    &= \frac{1}{\lambda}\Big(\vec{y}_0- 
    h(\vec{y}_0,\lambda)\int{\partiald{}{\vec{\theta}}\exp(\vec{\theta}\tp\vec{y}_0 - \lambda\psi(\vec{\theta}))}d\vec{\theta}\Big)\\
    &= \frac{1}{\lambda}\vec{y}_0-\frac{h(\vec{y}_0,\lambda)}{\lambda}
       \int{
           \partiald{}{\vec{\theta}}\exp(\vec{\theta}\tp\vec{y}_0 - \lambda\psi(\vec{\theta}))
       }d\vec{\theta}\\
\end{align*}

Since $\vec{y}\vert\vec{\theta}$ is distributed according to an exponential family distribution, $\expec{\vec{y}\vert\vec{\theta}} =\expec{\xi(\vec{\theta})}$ must exist.
Therefore, $\int{\partiald{}{\vec{\theta}}\exp(\vec{\theta}\tp\vec{y}_0 - \lambda\psi(\vec{\theta}))}d\vec{\theta}$ must converge.
Thus, 
\begin{align*}
     \frac{1}{\lambda}\vec{y}_0- 
\frac{h(\vec{y}_0,\lambda)}{\lambda}\int{\partiald{}{\vec{\theta}}\exp(\vec{\theta}\tp\vec{y}_0 - \lambda\psi(\vec{\theta}))}d\vec{\theta} = \frac{1}{\lambda}\vec{y}_0 + constant
\end{align*}


